Improve wp_to_wpc experiment

src/program_proof/wp_to_wpc.v
@@ -57,36 +57,54 @@ Definition N1 := N.@"1".
 Definition N2 := N.@"2".
 
 Definition mysch : bi_schema :=
-  (bi_sch_or (bi_sch_and (bi_sch_var_mut 0) (bi_sch_except_0 (bi_sch_var_fixed 0)))
+  (bi_sch_or (bi_sch_and (bi_sch_var_mut 0) (bi_sch_except_0 (bi_sch_fupd ∅ ∅ (bi_sch_var_fixed 0))))
              (bi_sch_var_fixed 1)).
 Lemma mysch_interp_weak k P Qs_mut γ :
-  bi_schema_interp k (bi_later <$> [P; staged_done γ]) (bi_later <$> Qs_mut) mysch ⊣⊢
+  bi_schema_interp (S k) (bi_later <$> [P; staged_done γ]) (bi_later <$> Qs_mut) mysch ⊣⊢
                    let Qs := default emp%I (bi_later <$> (Qs_mut !! O)) in
-                      (((Qs ∧ ◇ ▷ P) ∨ (▷ staged_done γ)))%I.
+                      (((Qs ∧ ◇ |k,Some O={∅}=> ▷ P) ∨ (▷ staged_done γ)))%I.
 Proof.
-  repeat (rewrite ?bi_schema_interp_unfold /= //=).
+  remember (S k) as n eqn:Heq.
+  do 2 (rewrite ?bi_schema_interp_unfold /= //=).
+  rewrite Heq.
+  erewrite (bi_sch_fupd_interp); last first.
+  { rewrite ?bi_schema_interp_unfold /= //=. }
+  rewrite /bi_sch_staged_fupd.
+  do 2 (rewrite ?bi_schema_interp_unfold /= //=).
   rewrite list_lookup_fmap. destruct (Qs_mut !! 0) => //=.
 Qed.
 
 Lemma mysch_interp_strong k P Q γ :
-  bi_schema_interp k (bi_later <$> [P; staged_done γ]) (bi_later <$> [Q]) mysch ⊣⊢
-                      (((▷ Q ∧ ◇ ▷ P) ∨ (▷ staged_done γ)))%I.
+  bi_schema_interp (S k) (bi_later <$> [P; staged_done γ]) (bi_later <$> [Q]) mysch ⊣⊢
+                      (((▷ Q ∧ ◇ |k,Some O={∅}=> ▷ P) ∨ (▷ staged_done γ)))%I.
 Proof.
-  repeat (rewrite ?bi_schema_interp_unfold /= //=).
+  remember (S k) as n eqn:Heq.
+  do 2 (rewrite ?bi_schema_interp_unfold /= //=).
+  rewrite Heq.
+  erewrite (bi_sch_fupd_interp); last first.
+  { rewrite ?bi_schema_interp_unfold /= //=. }
+  rewrite /bi_sch_staged_fupd.
+  do 2 (rewrite ?bi_schema_interp_unfold /= //=).
 Qed.
 
 Lemma wpc_spec P Φ Φc γ k E2:
   ↑N2 ⊆ E2 →
   is_foo1 N1 P γ ∗
-  (<bdisc> ▷ Φc ∧ (∀ σ, ▷ P σ ={⊤ ∖ ↑ N}=∗ ▷ P (transition σ) ∗ (<bdisc> ▷ Φc ∧ Φ (#())))) -∗
+  (<disc> ▷ Φc ∧ (∀ σ, ▷ P σ ={⊤ ∖ ↑ N}=∗ ▷ P (transition σ) ∗ (<disc> ▷ Φc ∧ Φ (#())))) -∗
   WPC e @ NotStuck; (S k); ⊤; E2 {{ Φ }} {{ Φc }}.
 Proof using stagedG0.
-iIntros (Hsub) "(His_foo&Hfupd)".
-rewrite and_comm.
+  iIntros (Hsub) "(His_foo&Hfupd)".
+  rewrite and_comm.
+  rewrite own_discrete_fupd_eq /own_discrete_fupd_def.
   iDestruct (own_discrete_elim_conj with "Hfupd") as (Q_keep Q_inv) "(HQ_keep&HQ_inv&#Hwand1&#Hwand2)".
   iMod (pending_alloc) as (γpending) "Hpending".
   iMod (inv_mut_alloc (S k) N2 _ mysch ([ Φc; staged_done γpending])%I [Q_inv] with "[HQ_inv]") as "(#Hinv&Hfull)".
-  { rewrite mysch_interp_strong. iLeft. iSplit; first auto. by iApply "Hwand1". }
+  { rewrite mysch_interp_strong. iLeft. iSplit; first auto.
+    iMod ("Hwand1" with "[$]") as "H".
+    iModIntro. iMod (fupd_level_split_level with "H") as "$".
+    { lia. }
+    eauto.
+  }
   iDestruct (pending_split with "Hpending") as "(Hpend1&Hpend2)".
   iAssert (WPC e @ S k; ⊤;∅ {{ v, staged_pending (1 / 2) γpending -∗ |={⊤}=> Φ v }} {{ True }})%I with "[His_foo HQ_keep Hpend1 Hfull]" as "Hwpc"; last first.
   {
@@ -99,7 +117,12 @@ rewrite and_comm.
     iMod (inv_mut_acc with "Hinv") as (Qs) "(H&Hclo)"; first auto.
     rewrite mysch_interp_weak /=.
     iDestruct "H" as "[(_&>H)|>Hfalse]".
-    * iApply fupd_level_mask_weaken; first set_solver+. eauto.
+    *
+      iEval (rewrite uPred_fupd_level_eq /uPred_fupd_level_def).
+      iMod (fupd_split_level_intro_mask' _ ∅) as "Hclo''"; first by set_solver+.
+      iMod (fupd_split_level_le with "H") as "H"; first lia.
+      iMod "Hclo''".
+      iApply fupd_split_level_mask_weaken; first set_solver+. eauto.
     * iDestruct (pending_done with "[$] [$]") as "[]".
   }
   iApply (wp_wpc).
@@ -120,7 +143,11 @@ rewrite and_comm.
   iDestruct (own_discrete_elim_conj with "HΦ") as (Q_keep' Q_inv') "(HQ_keep&HQ_inv&#Hwand1&#Hwand2)".
   iMod ("Hclo" $! [Q_inv'] with "[HQ_inv]") as "Hfull".
   { rewrite ?mysch_interp_strong. iLeft. iSplit; first auto.
-    by iApply "Hwand1". }
+    iMod ("Hwand1" with "[$]") as "H".
+    iModIntro. iMod (fupd_level_split_level with "H") as "$".
+    { lia. }
+    eauto.
+  }
   iModIntro.
   iFrame "HP". iModIntro. iIntros "Hpending".
   iDestruct (pending_join with "[$Hpending $Hpend1]") as "Hpend".
